vanilla_version/countability.v
@@ -1,4 +1,4 @@
-Require Import Utf8 Lia Arith Nat Setoid Morphisms Recdef utils basics.
+Require Import Utf8 List Lia Arith Nat Recdef EqdepFacts utils basics.
 Set Implicit Arguments.
 
 (* Cantor pairing function *)
@@ -37,87 +37,52 @@ Qed.
 
 (*-------*)
 
-Definition injective A B Ra Rb (Ea: @Equivalence A Ra) (Eb: @Equivalence B Rb) f (Hf: Proper (Ra ==> Rb) f) :=
-  ∀ x y, Rb (f x) (f y) → Ra x y.
-Definition bijective A B Ra Rb (Ea: @Equivalence A Ra) (Eb: @Equivalence B Rb)
-  f g (Hf: Proper (Ra ==> Rb) f) (Hg: Proper (Rb ==> Ra) g) :=
-  injective Ea Eb Hf ∧ injective Eb Ea Hg.
-Definition countable A R (E: @Equivalence A R) :=
-  ∃ f (Hf: Proper (R ==> eq) f), injective E (@eq_equivalence nat) Hf.
+Definition hinjective I (A: I → Type) (B: Type) (f: ∀ i, A i → B) := ∀ i x j y, f i x = f j y → eq_dep I A i x j y.
+Definition hcountable I (A: I → Type) := ∃ (f: ∀ i, A i → nat), hinjective A f.
 
-Definition compose A B C Ra Rb Rc (Ea: @Equivalence A Ra) (Eb: @Equivalence B Rb) (Ec: @Equivalence C Rc)
-  f g (Hf: Proper (Ra ==> Rb) f) (Hg: Proper (Rb ==> Rc) g):
-  Proper (Ra ==> Rc) (λ x, g (f x)).
-Proof.
-  intros ? ? ?. apply Hg. apply Hf. auto.
-Qed.
+Definition countable A := ∃ (f: A → nat), injective f.
 
-Definition compose_injective A B C Ra Rb Rc (Ea: @Equivalence A Ra) (Eb: @Equivalence B Rb) (Ec: @Equivalence C Rc)
-  f g (Hf: Proper (Ra ==> Rb) f) (Hg: Proper (Rb ==> Rc) g) (H: injective _ _ Hf) (H0: injective _ _ Hg):
-  injective Ea Ec (compose _ _ _ Hf Hg).
+Definition prod_countable A B (Ha: countable A) (Hb: countable B): countable (A * B)%type.
 Proof.
-  intros ? ? ?. apply H, H0. auto.
-Qed.
-
-Definition smaller_than_countable A B Ra Rb (Ea: @Equivalence A Ra) (Eb: @Equivalence B Rb)
-  f (Hf: Proper (Ra ==> Rb) f) (H: injective _ _ Hf) (H0: countable Eb):
-  countable Ea.
-Proof.
-  destruct H0 as [g [Hg H0]]. unfold countable. exists (Basics.compose g f), (compose _ _ _ Hf Hg).
-  apply (compose_injective H H0).
-Qed.
-
-Definition pair_eq A B (Ra: A → A → Prop) (Rb: B → B → Prop) :=
-  λ p1 p2, match p1, p2 with (x1, y1), (x2, y2) => Ra x1 x2 ∧ Rb y1 y2 end.
-Definition pair_Equivalence A B Ra Rb (Ea: @Equivalence A Ra) (Eb: @Equivalence B Rb):
-  @Equivalence _ (pair_eq Ra Rb).
-Proof.
-  split.
-  + intros ?. destruct x; simpl. split. apply Ea. apply Eb.
-  + intros ? ? ?. destruct x, y; simpl. destruct H; split. apply Ea. auto. apply Eb. auto.
-  + intros ? ? ? ? ?. destruct x, y, z; simpl. destruct H, H0; split. etransitivity; eauto. etransitivity; eauto.
-Qed.
-
-Definition prod_countable A B Ra Rb (Ea: @Equivalence A Ra) (Eb: @Equivalence B Rb)
-  (Ha: countable Ea) (Hb: countable Eb):
-  countable (pair_Equivalence Ea Eb).
-Proof.
-  destruct Ha as [fa [Ha H0]], Hb as [fb [Hb H1]].
+  destruct Ha as [fa Ha], Hb as [fb Hb].
   set (fun p => match p with (x, y) => Cantor_pairing (fa x, fb y) end) as f.
-  assert (Proper (pair_eq Ra Rb ==> eq) f).
-  { intros ? ? ?. destruct x, y. unfold f, pair_eq in *. destruct H.
-    f_equal. f_equal. apply Ha. auto. apply Hb. auto. }
-  exists f, H. intros ? ? ?. destruct x, y; simpl. unfold f in *.
+  exists f. intros ? ? ?. destruct x, y; simpl. unfold f in *.
   assert ((fa a, fb b) = Cantor_pairing_inv (Cantor_pairing (fa a0, fb b0))).
   { apply Cantor_pairing_inv_thm. auto. }
   assert ((fa a0, fb b0) = Cantor_pairing_inv (Cantor_pairing (fa a0, fb b0))).
   { apply Cantor_pairing_inv_thm. auto. }
   assert (fa a = fa a0) by congruence. assert (fb b = fb b0) by congruence.
-  apply H0 in H5. apply H1 in H6. auto.
+  apply Ha in H2. apply Hb in H3. congruence.
 Qed.
 
-Definition list_Equivalence A R (E: @Equivalence A R): Equivalence (List.Forall2 R).
+Definition sum_eq A B (Ra: A → A → Prop) (Rb: B → B → Prop): A + B → A + B → Prop.
 Proof.
-  split.
-  + intros ?. induction x; auto. constructor. reflexivity. auto.
-  + intros ?. induction x; intros.
-    - inversion H; subst; clear H. constructor.
-    - inversion H; subst; clear H. constructor. apply E; auto. eauto.
-  + intros ?. induction x; intros.
-    - inversion H; subst; clear H. inversion H0; subst; clear H0. constructor.
-    - inversion H; subst; clear H. inversion H0; subst; clear H0. constructor.
-      etransitivity; eauto. eapply IHx; eauto.
-Qed.
+  intros x y. destruct x as [xa | xb], y as [ya | yb].
+  + exact (Ra xa ya).
+  + exact False.
+  + exact False.
+  + exact (Rb xb yb).
+Defined.
 
-Theorem half_bijection_an_injection A B Ra Rb (Ea: @Equivalence A Ra) (Eb: @Equivalence B Rb)
-  f g (Hf: Proper (Ra ==> Rb) f) (Hg: Proper (Rb ==> Ra) g):
-  (∀ x, Ra (g (f x)) x) → injective Ea Eb Hf.
+Definition sum_countable A B (Ha: countable A) (Hb: countable B): countable (A + B).
 Proof.
-  intros H. unfold injective. intros x y H1. apply Hg in H1. do 2 rewrite H in H1. auto.
+  destruct Ha as [fa Ha], Hb as [fb Hb]. unfold countable.
+  refine (let f: A + B → nat := _ in _). Unshelve.
+  2:{ intro. destruct X. exact (fa a * 2). exact (S (fb b * 2)). }
+  exists f. intros ? ? ?. unfold f in *. destruct x, y; simpl in *.
+  + assert (fa a = fa a0) by lia. apply Ha in H0. congruence.
+  + lia.
+  + lia.
+  + assert (fb b = fb b0) by lia. apply Hb in H0. congruence.
+Qed.
+
+Theorem half_bijection_an_injection A B (f: A → B) (g: B → A): (∀ x, g (f x) = x) → injective f.
+Proof.
+  intros H. unfold injective. intros x y H0. congruence.
 Qed.
 
 
-Definition code (L: list nat) := List.fold_right (λ n m, (2 ^ n) * (S (m * 2))) 0 L.
+Definition encode_list (L: list nat) := List.fold_right (λ n m, (2 ^ n) * (S (m * 2))) 0 L.
 
 Function get_2_power (n: nat) { measure (λ x, x) } :=
   match n with
@@ -131,11 +96,11 @@ Proof.
   intros. apply Nat.div_lt; lia.
 Defined.
 
-Function decode (n: nat) { measure (λ x, x) } :=
+Function decode_list (n: nat) { measure (λ x, x) } :=
   match n with
   | O => nil
   | S m => let w := get_2_power n in
-           cons w (decode (n / (2 ^ S w)))
+           cons w (decode_list (n / (2 ^ S w)))
   end.
 Proof.
   intros. rewrite <- teq. rewrite Nat.pow_succ_r'. rewrite <- Nat.div_div; try lia.
@@ -149,7 +114,7 @@ Proof.
     assert (1 < 2 ^ S n0) by (apply Nat.pow_gt_1; lia). lia. }
 Defined.
 
-Theorem decode_code_thm (L: list nat): decode (code L) = L.
+Theorem decode_encode_list_thm (L: list nat): decode_list (encode_list L) = L.
 Proof.
   assert (∀ a w, get_2_power (2 ^ a * S (w * 2)) = a).
   { intros. induction a.
@@ -160,50 +125,55 @@ Proof.
       replace (S (_ * _ - 1)) with (2 ^ S a * S (w * 2)) by lia.
       rewrite Nat.pow_succ_r'. replace (2 * _ * _) with (2 ^ a * S (w * 2) * 2) by lia.
       rewrite Nat.mod_mul; try lia. rewrite Nat.div_mul; try lia. }
-  induction L; simpl; rewrite decode_equation; auto. destruct a.
-  + replace (2 ^ 0 * S (code L * 2)) with (S (code L * 2)) by (simpl; lia). f_equal.
-    - replace (S (code L * 2)) with (2 ^ 0 * S (code L * 2)) by (simpl; lia). rewrite H. auto.
-    - replace (S (code L * 2)) with (2 ^ 0 * S (code L * 2)) by (simpl; lia). rewrite H.
-      simpl (2 ^ 0)%nat. simpl (2 ^ 1)%nat. replace (1 * _) with (1 + code L * 2) by lia.
+  induction L; simpl; rewrite decode_list_equation; auto. destruct a.
+  + replace (2 ^ 0 * S (encode_list L * 2)) with (S (encode_list L * 2)) by (simpl; lia). f_equal.
+    - replace (S (encode_list L * 2)) with (2 ^ 0 * S (encode_list L * 2)) by (simpl; lia). rewrite H. auto.
+    - replace (S (encode_list L * 2)) with (2 ^ 0 * S (encode_list L * 2)) by (simpl; lia). rewrite H.
+      simpl (2 ^ 0)%nat. simpl (2 ^ 1)%nat. replace (1 * _) with (1 + encode_list L * 2) by lia.
       rewrite Nat.div_add; try lia. simpl. auto.
   + rewrite H. assert (1 < 2 ^ S a). { apply Nat.pow_gt_1; lia. }
-    replace (2 ^ S a * S (code L * 2)) with (S (2 ^ S a * S (code L * 2) - 1)) by lia. f_equal.
-    replace (S (_ - 1)) with (2 ^ S a * S (code L * 2)) by lia.
+    replace (2 ^ S a * S (encode_list L * 2)) with (S (2 ^ S a * S (encode_list L * 2) - 1)) by lia. f_equal.
+    replace (S (_ - 1)) with (2 ^ S a * S (encode_list L * 2)) by lia.
     repeat rewrite Nat.pow_succ_r'. replace (2 * (2 * 2 ^ a)) with (2 ^ a * 2 * 2) by lia.
-    repeat rewrite <- Nat.div_div; try lia. replace (_ * _ * _) with (S (code L * 2) * 2 * 2 ^ a) by lia.
-    repeat rewrite Nat.div_mul; try lia. replace (S _) with (1 + code L * 2) by lia.
+    repeat rewrite <- Nat.div_div; try lia. replace (_ * _ * _) with (S (encode_list L * 2) * 2 * 2 ^ a) by lia.
+    repeat rewrite Nat.div_mul; try lia. replace (S _) with (1 + encode_list L * 2) by lia.
     rewrite Nat.div_add; try lia. simpl. auto.
     { clear H0. induction a; simpl; try lia. }
     { clear H0. induction a; simpl; try lia. }
     { clear H0. induction a; simpl; try lia. }
 Qed.
 
-Definition lists_countable A R (E: @Equivalence A R) (H: countable E): countable (list_Equivalence E).
+Definition lists_countable A (H: countable A): countable (list A).
 Proof.
-  destruct H as [f [Hf H]]. set (λ L, code (List.map f L)) as F.
-  assert (Proper (List.Forall2 R ==> eq) F).
-  { intros ?. unfold F. induction x; simpl; intros.
-    + inversion H0; subst; clear H0. reflexivity.
-    + inversion H0; subst; clear H0. simpl. replace (f a) with (f y0).
-      rewrite (IHx l' H5). reflexivity. apply Hf; symmetry; auto. }
-  exists F, H0. intros ? ? ?. unfold F in *.
-  revert y H1. induction x; simpl; intros.
-  + assert (decode 0 = decode (code (List.map f y))) by congruence.
-    assert (decode 0 = nil) by (compute; auto). rewrite decode_code_thm in H2. rewrite H3 in H2.
-    symmetry in H2. apply List.map_eq_nil in H2. subst. constructor.
+  destruct H as [f Hf]. set (λ L, encode_list (map f L)) as F.
+  exists F. intros ? ? ?. unfold F in *.
+  revert y H. induction x; simpl; intros.
+  + assert (decode_list 0 = decode_list (encode_list (List.map f y))) by congruence.
+    assert (decode_list 0 = nil) by (compute; auto). rewrite decode_encode_list_thm in H0. rewrite H1 in H0.
+    symmetry in H0. apply List.map_eq_nil in H0. subst. auto.
   + destruct y.
-    - simpl in H1. assert (∀ w, 0 < 2 ^ w). { induction w; simpl; try lia. }
-      pose (H2 (f a)). lia.
-    - simpl in H1. assert (f a = f a0).
-      { revert H1. generalize (f a) as w1, (f a0) as w2. induction w1; simpl; intros.
-        + destruct w2; auto. simpl in H1. lia.
+    - simpl in H. assert (∀ w, 0 < 2 ^ w). { induction w; simpl; try lia. }
+      pose (H0 (f a)). lia.
+    - simpl in H. assert (f a = f a0).
+      { revert H. generalize (f a) as w1, (f a0) as w2. induction w1; simpl; intros.
+        + destruct w2; auto. simpl in H. lia.
         + destruct w2.
-          - simpl in H1. lia.
-          - simpl in H1. f_equal. apply IHw1. lia. }
-      constructor.
-      * apply H. auto.
-      * rewrite H2 in H1. apply Nat.mul_cancel_l in H1.
+          - simpl in H. lia.
+          - simpl in H. f_equal. apply IHw1. lia. }
+      f_equal.
+      * apply Hf. auto.
+      * rewrite H0 in H. apply Nat.mul_cancel_l in H.
         ++ apply IHx. lia.
         ++ generalize (f a0) as w. induction w; simpl; lia.
 Qed.
+
+
+Definition encode_Term F R V (L: Language F R) (T: Term V L): list (F + V).
+Proof.
+  destruct T. clear e. induction x using preTerm_recursion; simpl in *.
+  + exact (inr v :: nil).
+  + induction v.
+    - exact nil.
+    - inversion X; subst; clear X. exact (IHv X1 ++ X0).
+Defined.
 
