mathcomp_version/countability.v
@@ -1,0 +1,7 @@
+From mathcomp Require Import all_ssreflect.
+Require Import Utf8 basics.
+Import EqNotations.
+Set Implicit Arguments.
+
+
+
